BLAKE2 round soundness proof

Clean/Gadgets/BLAKE3/Round.lean
@@ -20,18 +20,18 @@ instance : ProvableStruct Inputs where
 
 def main (input : Var Inputs (F p)) : Circuit (F p) (Var BLAKE3State (F p)) := do
   let { state, message } := input
-  .foldl (_const_out := by
-    rintro ⟨inputs, a, b, c, d, i, j, h_j⟩
-    intro i0
-    simp [circuit_norm, G.circuit]
-    --TODO: this is not trivial because the output depends on a b c d.
-    -- however, the `roundConstants` are fixed, so morally they are constants
-    sorry
-  ) roundConstants state
-    fun state (a, b, c, d, i, j) => subcircuit (G.circuit a b c d) ⟨state, message[i], message[j]⟩
+  let state ← subcircuit (G.circuit 0 4 8 12) ⟨state, message[0], message[1]⟩
+  let state ← subcircuit (G.circuit 1 5 9 13) ⟨state, message[2], message[3]⟩
+  let state ← subcircuit (G.circuit 2 6 10 14) ⟨state, message[4], message[5]⟩
+  let state ← subcircuit (G.circuit 3 7 11 15) ⟨state, message[6], message[7]⟩
+  let state ← subcircuit (G.circuit 0 5 10 15) ⟨state, message[8], message[9]⟩
+  let state ← subcircuit (G.circuit 1 6 11 12) ⟨state, message[10], message[11]⟩
+  let state ← subcircuit (G.circuit 2 7 8 13) ⟨state, message[12], message[13]⟩
+  let state ← subcircuit (G.circuit 3 4 9 14) ⟨state, message[14], message[15]⟩
+  return state
 
--- #eval! main (p:=p_babybear) default |>.local_length
--- #eval! main (p:=p_babybear) default |>.output
+-- #eval! main (p:=pBabybear) default |>.localLength
+-- #eval! main (p:=pBabybear) default |>.output
 instance elaborated : ElaboratedCircuit (F p) Inputs BLAKE3State where
   main := main
   localLength _ := 768
@@ -50,9 +50,38 @@ theorem soundness : Soundness (F p) elaborated Assumptions Spec := by
   intro i0 env ⟨state_var, message_var⟩ ⟨state, message⟩ h_input h_normalized h_holds
   simp only [circuit_norm, Inputs.mk.injEq] at h_input
 
-  simp [circuit_norm, subcircuit_norm, main, G.elaborated, G.circuit] at h_holds
+  dsimp [Assumptions] at h_normalized
+  obtain ⟨h_state, h_message⟩ := h_normalized
+  obtain ⟨h_eval_state, h_eval_message⟩ := h_input
 
-  sorry
+  dsimp [circuit_norm, subcircuit_norm, main, G.elaborated, G.circuit, Rotation32.output] at h_holds
+  simp [h_eval_state, h_eval_message, G.Spec, circuit_norm, getElem_eval_vector, G.Assumptions] at h_holds
+  obtain ⟨c1, c2, c3, c4, c5, c6, c7, c8⟩ := h_holds
+  simp_all only [forall_const]
+
+  specialize c1 (h_message 0) (h_message 1)
+  rw [c1.left] at c2
+  specialize c2 c1.right (h_message 2) (h_message 3)
+  rw [c2.left] at c3
+  specialize c3 c2.right (h_message 4) (h_message 5)
+  rw [c3.left] at c4
+  specialize c4 c3.right (h_message 6) (h_message 7)
+  rw [c4.left] at c5
+  specialize c5 c4.right (h_message 8) (h_message 9)
+  rw [c5.left] at c6
+  specialize c6 c5.right (h_message 10) (h_message 11)
+  rw [c6.left] at c7
+  specialize c7 c6.right (h_message 12) (h_message 13)
+  rw [c7.left] at c8
+  specialize c8 c7.right (h_message 14) (h_message 15)
+
+  clear c1 c2 c3 c4 c5 c6 c7
+
+  simp [Spec, circuit_norm, main, subcircuit_norm, elaborated, G.elaborated, G.circuit,
+    Specs.BLAKE3.round, Vector.foldl, roundConstants, circuit_norm]
+  constructor
+  · rw [←c8.left]; rfl
+  · exact c8.right
 
 theorem completeness : Completeness (F p) elaborated Assumptions := by
   rintro i0 env input_var henv input h_input h_normalized
